Resource template OK

Phi_Algebras/Phi_Fiction_2.thy
@@ -1,5 +1,5 @@
-theory Phi_Fiction
-  imports Phi_Algebra_Set Unital_Homo
+theory Phi_Fiction_2
+  imports Algebras
 begin
 
 section \<open>Interpretation of Fictional Separation\<close>
@@ -26,9 +26,28 @@ text \<open>
   maps a fictional resource to a set of concrete resource.
   The interpretation can be any map to set that preserves \<open>1\<close>, the unit of the separation algebra.\<close>
 
+definition Interpretation :: "('a::one \<Rightarrow> 'b::one set) \<Rightarrow> bool"
+  where "Interpretation \<I> \<longleftrightarrow> \<I> 1 = 1"
 
-type_synonym ('a,'b) interp = \<open>'a \<Rightarrow> 'b set\<close>
-type_synonym ('a,'b) unital_homo_interp = \<open>('a, 'b set) unital_homo\<close>
+typedef (overloaded) ('a::one,'b::one) interp
+    = \<open>Collect (Interpretation :: ('a \<Rightarrow> 'b set) \<Rightarrow> bool)\<close>
+  morphisms \<I> Interp
+  by (rule exI[where x = \<open>\<lambda>_. 1\<close>]) (simp add:sep_mult_commute Interpretation_def)
+
+text \<open>Type \<open>('a,'b) interp\<close> encapsulating the 1-preserving condition, represents an interpretation.
+\<^const>\<open>\<I>\<close> activates the interpretation; \<^const>\<open>Interp\<close> constructs an interpretation by checking
+the 1-preserving condition.
+\[@{thm Interp_inverse[simplified]}\]\<close>
+
+lemmas Interp_inverse[simp] = Interp_inverse[simplified]
+
+lemma Interp_one[simp]: "\<I> I 1 = 1"
+  using Interpretation_def \<I> by blast
+
+lemma interp_eq_I[intro!]:
+  \<open>\<I> x = \<I> y \<Longrightarrow> x = y\<close>
+  by (simp add: \<I>_inject)
+  
 
 (*
 definition \<I>\<^sub>r\<^sub>e\<^sub>l :: \<open>('a::one,'b::one) interp \<Rightarrow> ('a \<times> 'b) set\<close> 
@@ -37,10 +56,10 @@ definition \<I>\<^sub>r\<^sub>e\<^sub>l :: \<open>('a::one,'b::one) interp \<Rig
 
 subsubsection \<open>Fictional Refinement\<close>
 
-definition Fictional_Forward_Simulation :: \<open>'c rel \<Rightarrow> 'a rel \<Rightarrow> ('a::sep_magma,'c::sep_magma) interp \<Rightarrow> 'a set \<Rightarrow> bool\<close>
+definition Fictional_Forward_Simulation :: \<open>'c rel \<Rightarrow> 'a rel \<Rightarrow> ('a::sep_magma_1,'c::sep_magma_1) interp \<Rightarrow> 'a set \<Rightarrow> bool\<close>
       ("_/ \<r>\<e>\<f>\<i>\<n>\<e>\<s> _/ \<w>.\<r>.\<t> _/ \<i>\<n> _" [11,11,11] 10)
   where \<open>(F \<r>\<e>\<f>\<i>\<n>\<e>\<s> G \<w>.\<r>.\<t> T \<i>\<n> D)
-    \<longleftrightarrow> (\<forall>x r R. F `` (R * T (r * x) \<s>\<u>\<b>\<j> r ## x \<and> x \<in> D) \<subseteq> { y'. \<exists>y. y' \<in> R * T (r * y) \<and> r ## y \<and> (x,y) \<in> G})\<close>
+    \<longleftrightarrow> (\<forall>x r R. F `` (R * \<I> T (r * x) \<s>\<u>\<b>\<j> r ## x \<and> x \<in> D) \<subseteq> { y'. \<exists>y. y' \<in> R * \<I> T (r * y) \<and> r ## y \<and> (x,y) \<in> G})\<close>
 
 text \<open>We use relation directly here but doesn't mean we cannot model return value or threw exceptions.
 They can parameterize the relation, as we don't need to (it is not designed to) abstract the values.
@@ -48,6 +67,8 @@ We only relate resources in different abstractions.
 
 \<^prop>\<open>\<And>ret. F ret \<r>\<e>\<f>\<i>\<n>\<e>\<s> G ret \<w>.\<r>.\<t> T \<i>\<n> D\<close>
 \<close>
+
+definition \<open>refinement_projection I D = \<Union> (\<I> I ` (UNIV * D))\<close>
 
 lemma empty_refines_any[simp]:
   \<open>{} \<r>\<e>\<f>\<i>\<n>\<e>\<s> Any \<w>.\<r>.\<t> I \<i>\<n> D\<close>
@@ -78,7 +99,7 @@ lemma refinement_sub_fun_right:
 lemma refinement_frame:
   \<open> A \<r>\<e>\<f>\<i>\<n>\<e>\<s> B \<w>.\<r>.\<t> I \<i>\<n> D
 \<Longrightarrow> A \<r>\<e>\<f>\<i>\<n>\<e>\<s> Id_on R * B \<w>.\<r>.\<t> I \<i>\<n> R * D\<close>
-  for B :: \<open>'b::sep_semigroup rel\<close>
+  for B :: \<open>'b::sep_monoid rel\<close>
   unfolding Fictional_Forward_Simulation_def
   apply (clarsimp simp add: subset_iff Subjection_expn set_mult_expn Image_def Bex_def Id_on_iff)
   by (smt (z3) sep_disj_multD1 sep_disj_multD2 sep_disj_multI1 sep_disj_multI2 sep_mult_assoc')
@@ -92,7 +113,7 @@ lemma sep_refinement_horizontal_stepwise:
   apply (clarsimp simp add: set_mult_expn Subjection_expn subset_iff Image_def Bex_def)
   subgoal premises prems for x r R u v y z
   proof -
-    have \<open>(\<exists>xa. (\<exists>u v. xa = u * v \<and> u \<in> R \<and> v \<in> I (r * x) \<and> u ## v) \<and> r ## x \<and> x \<in> D \<and> (xa, y) \<in> A1)\<close>
+    have \<open>(\<exists>xa. (\<exists>u v. xa = u * v \<and> u \<in> R \<and> v \<in> \<I> I (r * x) \<and> u ## v) \<and> r ## x \<and> x \<in> D \<and> (xa, y) \<in> A1)\<close>
       using prems(10) prems(4) prems(5) prems(6) prems(8) prems(9) by blast
     note prems(1)[THEN spec[where x=x], THEN spec[where x=r], THEN spec[where x=R], THEN spec[where x=y],
           THEN mp, OF this]
@@ -100,7 +121,7 @@ lemma sep_refinement_horizontal_stepwise:
       apply clarsimp
       subgoal premises prems2 for y' u' v'
       proof -
-        have \<open>(\<exists>x. (\<exists>u v. x = u * v \<and> u \<in> R \<and> v \<in> I (r * y') \<and> u ## v) \<and> r ## y' \<and> y' \<in> D' \<and> (x, z) \<in> A2)\<close>
+        have \<open>(\<exists>x. (\<exists>u v. x = u * v \<and> u \<in> R \<and> v \<in> \<I> I (r * y') \<and> u ## v) \<and> r ## y' \<and> y' \<in> D' \<and> (x, z) \<in> A2)\<close>
           using prems(3) prems(5) prems(7) prems2(1) prems2(2) prems2(3) prems2(4) prems2(5) prems2(6) by blast
         note prems(2)[THEN spec[where x=y'], THEN spec[where x=r], THEN spec[where x=R], THEN spec[where x=z],
           THEN mp, OF this]
@@ -116,22 +137,10 @@ lemma constant_refinement:
   by (clarsimp simp add: subset_iff Id_on_iff set_mult_expn Subjection_expn times_fun; blast)
 
 lemma refinement_subjection:
-  \<open> (P \<Longrightarrow> A \<r>\<e>\<f>\<i>\<n>\<e>\<s> B \<w>.\<r>.\<t> I \<i>\<n> D)
-\<Longrightarrow> P \<longrightarrow> Q
-\<Longrightarrow> A \<s>\<u>\<b>\<j> P \<r>\<e>\<f>\<i>\<n>\<e>\<s> B \<s>\<u>\<b>\<j> Q \<w>.\<r>.\<t> I \<i>\<n> D\<close>
+  \<open> A \<r>\<e>\<f>\<i>\<n>\<e>\<s> B \<w>.\<r>.\<t> I \<i>\<n> D
+\<Longrightarrow> A \<s>\<u>\<b>\<j> P \<r>\<e>\<f>\<i>\<n>\<e>\<s> B \<s>\<u>\<b>\<j> P \<w>.\<r>.\<t> I \<i>\<n> D\<close>
   unfolding Fictional_Forward_Simulation_def
   by (clarsimp simp add: Subjection_expn subset_iff Image_def Bex_def Id_on_iff)
-
-lemma refinement_existential:
-  \<open> (\<And>x. A x \<r>\<e>\<f>\<i>\<n>\<e>\<s> B x \<w>.\<r>.\<t> I \<i>\<n> D)
-\<Longrightarrow> ExSet A \<r>\<e>\<f>\<i>\<n>\<e>\<s> ExSet B \<w>.\<r>.\<t> I \<i>\<n> D\<close>
-  unfolding Fictional_Forward_Simulation_def
-  by (clarsimp simp add: Subjection_expn ExSet_expn subset_iff Image_def Bex_def Id_on_iff; blast)
-
-lemma refinement_source_subjection:
-  \<open>(A \<s>\<u>\<b>\<j> P \<r>\<e>\<f>\<i>\<n>\<e>\<s> B \<w>.\<r>.\<t> I \<i>\<n> D) \<longleftrightarrow> (P \<longrightarrow> (A \<r>\<e>\<f>\<i>\<n>\<e>\<s> B \<w>.\<r>.\<t> I \<i>\<n> D))\<close>
-  unfolding Fictional_Forward_Simulation_def
-  by (auto simp add: Subjection_expn subset_iff Image_def Bex_def Id_on_iff set_mult_expn; blast)
 
 lemma refinement_ExSet:
   \<open> (\<And>v. A v \<r>\<e>\<f>\<i>\<n>\<e>\<s> B v \<w>.\<r>.\<t> I \<i>\<n> D)
@@ -140,39 +149,26 @@ lemma refinement_ExSet:
   by (clarsimp simp add: ExSet_expn subset_iff Image_def Bex_def Id_on_iff, blast)
 
 
-definition \<open>refinement_projection I D = \<Union> (I ` (UNIV * D))\<close>
-
-lemma refinement_projection_mono:
-  \<open> D \<subseteq> D'
-\<Longrightarrow> refinement_projection I D \<subseteq> refinement_projection I D'\<close>
-  unfolding refinement_projection_def
-  by (clarsimp simp add: set_mult_expn Bex_def; blast)
-
-lemma UNIV_times_idem:
-  \<open>UNIV * UNIV = (UNIV :: 'a::sep_magma_1 set)\<close>
-  unfolding set_eq_iff
-  by (clarsimp simp add: set_mult_expn, metis mult_1_class.mult_1_right sep_magma_1_left)
-
-lemma refinement_projection_UNIV_times_D[simp]:
-  \<open> refinement_projection I (UNIV * D) = refinement_projection I D \<close>
-  for D :: \<open>'a::sep_monoid set\<close>
-  unfolding refinement_projection_def mult.assoc[symmetric] UNIV_times_idem ..
-
 subsection \<open>Instances\<close>
 
 subsubsection \<open>Identity\<close>
 
-definition [simp]: "\<F>_it x = {x}"
+definition [simp]: "\<F>_it' x = {x}"
+
+definition "\<F>_it = Interp \<F>_it'"
+
+lemma \<F>_it_\<I>[simp]: "\<I> \<F>_it = \<F>_it'"
+  unfolding \<F>_it_def
+  by (rule Interp_inverse) (simp add: Interpretation_def one_set_def)
 
 lemma \<F>_it_refinement_projection:
-  \<open> S \<subseteq> S'
-\<Longrightarrow> refinement_projection \<F>_it S \<subseteq> UNIV * S'\<close>
+  \<open>refinement_projection \<F>_it S \<subseteq> UNIV * S\<close>
   unfolding refinement_projection_def
   by (clarsimp simp add: set_mult_expn)
 
 lemma \<F>_it_refinement:
   \<open>Id_on UNIV * {(u,v)} \<r>\<e>\<f>\<i>\<n>\<e>\<s> {(u,v)} \<w>.\<r>.\<t> \<F>_it \<i>\<n> {u}\<close>
-  for u :: \<open>'a::{sep_cancel,sep_semigroup}\<close>
+  for u :: \<open>'a::{sep_cancel,sep_monoid}\<close>
   unfolding Fictional_Forward_Simulation_def
   by (clarsimp simp add: Subjection_expn set_mult_expn,
       metis sep_cancel sep_disj_multD1 sep_disj_multD2 sep_disj_multI1 sep_disj_multI2 sep_mult_assoc')
@@ -181,41 +177,44 @@ lemma \<F>_it_refinement:
 subsubsection \<open>Composition\<close>
 
 definition interp_comp :: \<open>('b::one,'c::one) interp \<Rightarrow> ('a::one,'b) interp \<Rightarrow> ('a,'c) interp\<close> (infixr "\<Zcomp>\<^sub>\<I>" 55)
-  where [simp]: \<open>(I1 \<Zcomp>\<^sub>\<I> I2) x = \<Union>(I1 ` I2 x)\<close>
+  where \<open>(I1 \<Zcomp>\<^sub>\<I> I2) = Interp (\<lambda>x. \<Union>(\<I> I1 ` \<I> I2 x))\<close>
+
+notation (ASCII) interp_comp  (infixl ";\<^sub>\<I>" 55)
+
+lemma interp_comp_\<I>[simp]:
+  \<open>\<I> (I1 \<Zcomp>\<^sub>\<I> I2) = (\<lambda>x. \<Union>(\<I> I1 ` \<I> I2 x))\<close>
+  unfolding interp_comp_def
+  by (rule Interp_inverse)  (simp add: Interpretation_def one_set_def)
 
 lemma interp_comp_assoc:
   \<open>(I1 \<Zcomp>\<^sub>\<I> I2) \<Zcomp>\<^sub>\<I> I3 = I1 \<Zcomp>\<^sub>\<I> (I2 \<Zcomp>\<^sub>\<I> I3)\<close>
-  by (simp add: fun_eq_iff)
-
-lemma interp_comp_homo_one[simp]:
-  \<open>homo_one Ia \<Longrightarrow> homo_one Ib \<Longrightarrow> homo_one (Ia \<Zcomp>\<^sub>\<I> Ib)\<close>
-  unfolding homo_one_def by (simp add: set_eq_iff)
+  by (subst \<I>_inject[symmetric]; simp)
 
 lemma \<F>_it_comp[simp]:
-  \<open>\<F>_it \<Zcomp>\<^sub>\<I> I = I\<close> \<open>I \<Zcomp>\<^sub>\<I> \<F>_it = I\<close>
-  by (simp add: fun_eq_iff)+
+  \<open>\<F>_it ;\<^sub>\<I> I = I\<close> \<open>I ;\<^sub>\<I> \<F>_it = I\<close>
+  by (subst \<I>_inject[symmetric], simp)+
 
 lemma sep_refinement_stepwise:
-  \<open> S1 \<r>\<e>\<f>\<i>\<n>\<e>\<s> S2 \<w>.\<r>.\<t> Ia \<i>\<n> D
-\<Longrightarrow> S2 \<r>\<e>\<f>\<i>\<n>\<e>\<s> S3 \<w>.\<r>.\<t> Ib \<i>\<n> D'
-\<Longrightarrow> refinement_projection Ib D' \<subseteq> D
-\<Longrightarrow> S1 \<r>\<e>\<f>\<i>\<n>\<e>\<s> S3 \<w>.\<r>.\<t> (Ia \<Zcomp>\<^sub>\<I> Ib) \<i>\<n> D'\<close>
-  for Ia :: \<open>'b::sep_magma_1 \<Rightarrow> 'a::sep_magma_1 set\<close>
-  unfolding Fictional_Forward_Simulation_def refinement_projection_def
+  \<open> S1 \<r>\<e>\<f>\<i>\<n>\<e>\<s> S2 \<w>.\<r>.\<t> I1 \<i>\<n> D
+\<Longrightarrow> S2 \<r>\<e>\<f>\<i>\<n>\<e>\<s> S3 \<w>.\<r>.\<t> I2 \<i>\<n> D'
+\<Longrightarrow> refinement_projection I2 D' \<subseteq> D
+\<Longrightarrow> S1 \<r>\<e>\<f>\<i>\<n>\<e>\<s> S3 \<w>.\<r>.\<t> (I1 \<Zcomp>\<^sub>\<I> I2) \<i>\<n> D'\<close>
+  unfolding Fictional_Forward_Simulation_def interp_comp_\<I> refinement_projection_def
   apply (auto simp add: subset_iff Image_def Bex_def Subjection_expn set_mult_expn split_option_all)
   subgoal premises prems for x r R t u v xb
   proof -
     thm prems
     thm prems(1)[THEN spec[where x=xb],THEN spec[where x=1],THEN spec[where x=\<open>R\<close>],THEN spec[where x=\<open>t\<close>]]
-    have \<open>(\<exists>x. (\<exists>u v. x = u * v \<and> u \<in> R \<and> v \<in> Ia (1 * xb) \<and> u ## v) \<and> 1 ## xb \<and> xb \<in> D \<and> (x, t) \<in> S1)\<close>
-      using prems(10) prems(3) prems(4) prems(5) prems(6) prems(7) prems(8) prems(9) by fastforce
+    have \<open>(\<exists>x. (\<exists>u v. x = u * v \<and> u \<in> R \<and> v \<in> \<I> I1 (1 * xb) \<and> u ## v) \<and> 1 ## xb \<and> xb \<in> D \<and> (x, t) \<in> S1)\<close>
+      apply (simp add: prems)
+      using prems(10) prems(3) prems(4) prems(5) prems(6) prems(7) prems(8) prems(9) by blast
     note prems(1)[THEN spec[where x=xb],THEN spec[where x=1],THEN spec[where x=\<open>R\<close>],THEN spec[where x=\<open>t\<close>],
           THEN mp, OF this]
     then show ?thesis
       apply clarsimp
       subgoal premises prems2 for y u'' v''
       proof -
-        have \<open>(\<exists>xa. (\<exists>u v. xa = u * v \<and> u \<in> {1} \<and> v \<in> Ib (r * x) \<and> u ## v) \<and> r ## x \<and> x \<in> D' \<and> (xa, y) \<in> S2)\<close>
+        have \<open>(\<exists>xa. (\<exists>u v. xa = u * v \<and> u \<in> {1} \<and> v \<in> \<I> I2 (r * x) \<and> u ## v) \<and> r ## x \<and> x \<in> D' \<and> (xa, y) \<in> S2)\<close>
           by (simp, rule exI[where x=xb], simp add: prems2 prems)
         note prems(2)[THEN spec[where x=x],THEN spec[where x=r],THEN spec[where x=\<open>{1}\<close>], THEN spec[where x=y],
                 THEN mp, OF this]
@@ -226,57 +225,37 @@ lemma sep_refinement_stepwise:
   qed .
 
 lemma sep_refinement_stepwise':
-  \<open> S1 \<r>\<e>\<f>\<i>\<n>\<e>\<s> S2 \<w>.\<r>.\<t> Ia \<i>\<n> D
-\<Longrightarrow> S2' \<r>\<e>\<f>\<i>\<n>\<e>\<s> S3 \<w>.\<r>.\<t> Ib \<i>\<n> D'
-\<Longrightarrow> refinement_projection Ib D' \<subseteq> D
+  \<open> S1 \<r>\<e>\<f>\<i>\<n>\<e>\<s> S2 \<w>.\<r>.\<t> I1 \<i>\<n> D
+\<Longrightarrow> S2' \<r>\<e>\<f>\<i>\<n>\<e>\<s> S3 \<w>.\<r>.\<t> I2 \<i>\<n> D'
+\<Longrightarrow> refinement_projection I2 D' \<subseteq> D
 \<Longrightarrow> S2 \<subseteq> S2'
-\<Longrightarrow> S1 \<r>\<e>\<f>\<i>\<n>\<e>\<s> S3 \<w>.\<r>.\<t> (Ia \<Zcomp>\<^sub>\<I> Ib) \<i>\<n> D'\<close>
-  for Ia :: \<open>'b::sep_magma_1 \<Rightarrow> 'a::sep_magma_1 set\<close>
+\<Longrightarrow> S1 \<r>\<e>\<f>\<i>\<n>\<e>\<s> S3 \<w>.\<r>.\<t> (I1 \<Zcomp>\<^sub>\<I> I2) \<i>\<n> D'\<close>
   using refinement_sub_fun sep_refinement_stepwise
   by metis
 
 lemma refinement_projections_stepwise:
-  \<open>refinement_projection (Ia \<Zcomp>\<^sub>\<I> Ib) D \<subseteq> refinement_projection Ia (refinement_projection Ib D)\<close>
-  for Ia :: \<open>('c::sep_monoid, 'a::sep_magma_1) interp\<close>
+  \<open>refinement_projection (I1 \<Zcomp>\<^sub>\<I> I2) D \<subseteq> refinement_projection I1 (refinement_projection I2 D)\<close>
+  for I1 :: \<open>('c::sep_monoid, 'a::sep_magma_1) interp\<close>
   unfolding refinement_projection_def
   apply (clarsimp simp add: Bex_def set_eq_iff set_mult_expn)
   subgoal for x x' u v
     by (metis mult_1_class.mult_1_left sep_magma_1_right) .
 
-lemma refinement_projections_stepwise_UNIV_paired:
-  \<open> refinement_projection Ia Da \<subseteq> UNIV * Dc
-\<Longrightarrow> refinement_projection Ib Db \<subseteq> UNIV * Da
-\<Longrightarrow> refinement_projection (Ia \<Zcomp>\<^sub>\<I> Ib) Db \<subseteq> UNIV * Dc\<close>
-  for Ia :: \<open>('c::sep_monoid, 'a::sep_magma_1) interp\<close>
-  using refinement_projections_stepwise
-  by (metis (mono_tags, lifting) refinement_projection_UNIV_times_D refinement_projection_mono subset_trans)
-
-
 subsubsection \<open>Function, pointwise\<close>
 
-definition [simp]: "\<F>_finite_product I f = prod (\<lambda>x. I x (f x)) (dom1 f)"
+definition "\<F>_fun' I = Interp (\<lambda>f. prod (\<lambda>x. \<I> (I x) (f x)) (dom1 f))"
 
-lemma \<F>_finite_product_split:
+lemma \<F>_fun'_\<I>[simp]: "\<I> (\<F>_fun' I) = (\<lambda>f. prod (\<lambda>x. \<I> (I x) (f x)) (dom1 f))"
+  unfolding \<F>_fun'_def by (rule Interp_inverse) (simp add: Interpretation_def)
+
+lemma \<F>_fun'_split:
   " finite (dom1 f)
-\<Longrightarrow> (\<And>k. homo_one (I k))
-\<Longrightarrow> \<F>_finite_product I f = \<F>_finite_product I (f(k:=1)) * I k (f k)
-   \<and> \<F>_finite_product I (f(k:=1)) ## I k (f k)"
-  for I :: \<open>'a \<Rightarrow> 'b::sep_algebra \<Rightarrow> 'c::sep_algebra set\<close>
-  by (simp add: homo_one_def,
-      smt (verit, best) dom1_upd fun_upd_triv mult.comm_neutral mult.commute prod.insert_remove)
+\<Longrightarrow> \<I> (\<F>_fun' I) f = \<I> (\<F>_fun' I) (f(k:=1)) * \<I> (I k) (f k)
+   \<and> \<I> (\<F>_fun' I) (f(k:=1)) ## \<I> (I k) (f k)"
+  for f :: "'a \<Rightarrow> 'b::sep_algebra"
+  by simp (smt (verit, best) Interp_one dom1_upd fun_upd_triv mult.comm_neutral mult.commute prod.insert_remove)
 
 
-definition [simp]: "\<F>_FP_homo I f = prod (\<lambda>x. apply_unital_homo (I x) (f x)) (dom1 f)"
-
-lemma \<F>_FP_homo_split:
-  " finite (dom1 f)
-\<Longrightarrow> \<F>_FP_homo I f = \<F>_FP_homo I (f(k:=1)) * apply_unital_homo (I k) (f k)
-   \<and> \<F>_FP_homo I (f(k:=1)) ## apply_unital_homo (I k) (f k)"
-  for I :: \<open>'a \<Rightarrow> ('b::sep_algebra, 'c::sep_algebra set) unital_homo\<close>
-  by (simp add: homo_one_def,
-      smt (verit, ccfv_SIG) Diff_empty Diff_insert0 apply_unital_homo_1 dom1_def mem_Collect_eq mult.commute mult_1_class.mult_1_right prod.remove)
-
-(*
 definition "\<F>_fun I = \<F>_fun' (\<lambda>_. I)"
 
 lemma \<F>_fun_\<I>[simp]: "\<I> (\<F>_fun I) = (\<lambda>f. prod (\<I> I o f) (dom1 f))"
@@ -290,8 +269,8 @@ lemma \<F>_fun_split:
   unfolding \<F>_fun_def using \<F>_fun'_split .
 
 lemma \<F>_interp_fun_\<I>_1_fupdt[simp]: "\<I> (\<F>_fun I) (1(k:=v)) = \<I> I v" by simp
-*)
-(*
+
+
 definition "\<F>_pointwise I = Interp (\<lambda>f. {g. \<forall>x. g x \<in> \<I> I (f x) })"
 
 lemma \<F>_pointwise_\<I>[simp]:
@@ -301,16 +280,17 @@ lemma \<F>_pointwise_\<I>[simp]:
 
 lemma \<F>_pointwise_\<F>_it:
   \<open>\<F>_pointwise \<F>_it = \<F>_it\<close>
-  by (rule interp_eq_I; simp add: fun_eq_iff set_eq_iff) *)
+  by (rule interp_eq_I; simp add: fun_eq_iff set_eq_iff)
 
-definition [simp]: "\<F>_pointwise I f = {g. \<forall>x. g x \<in> (I x) (f x)}"
+definition "\<F>_pointwise' I = Interp (\<lambda>f. {g. \<forall>x. g x \<in> \<I> (I x) (f x) })"
 
-lemma \<F>_pointwise_\<F>_it:
-  \<open>\<F>_pointwise (\<lambda>_. \<F>_it) = \<F>_it\<close>
-  by (simp add: fun_eq_iff set_eq_iff)
+lemma \<F>_pointwise'_\<I>[simp]:
+  "\<I> (\<F>_pointwise' I) = (\<lambda>f. {g. \<forall>x. g x \<in> \<I> (I x) (f x) })"
+  unfolding \<F>_pointwise'_def
+  by (rule Interp_inverse) (auto simp add: Interpretation_def one_fun_def fun_eq_iff)
 
 lemma \<F>_pointwise_projection:
-  \<open> refinement_projection (I k) D' \<subseteq> UNIV * D
+  \<open> refinement_projection I D' \<subseteq> UNIV * D
 \<Longrightarrow> refinement_projection (\<F>_pointwise I) (fun_upd 1 k ` D') \<subseteq> UNIV * fun_upd 1 k ` D\<close>
   for D :: \<open>'b::sep_monoid set\<close>
   apply (clarsimp simp add: subset_iff Bex_def image_iff set_mult_expn times_fun
@@ -319,7 +299,7 @@ lemma \<F>_pointwise_projection:
   proof -
     have t1: \<open>u k ## xb\<close>
       by (metis fun_upd_same prems(3) sep_disj_fun)
-    have \<open>(\<exists>x. (\<exists>xa. (\<exists>u v. xa = u * v \<and> v \<in> D' \<and> u ## v) \<and> x = I k xa) \<and> t k \<in> x)\<close>
+    have \<open>(\<exists>x. (\<exists>xa. (\<exists>u v. xa = u * v \<and> v \<in> D' \<and> u ## v) \<and> x = \<I> I xa) \<and> t k \<in> x)\<close>
       by (metis prems(2) prems(4) t1)
     note prems(1)[THEN spec[where x=\<open>t k\<close>], THEN mp, OF this]
     then show ?thesis
@@ -330,10 +310,9 @@ lemma \<F>_pointwise_projection:
   qed .
 
 lemma \<F>_pointwise_refinement:
-  \<open> Id_on UNIV * A \<r>\<e>\<f>\<i>\<n>\<e>\<s> B \<w>.\<r>.\<t> I k \<i>\<n> D
+  \<open> Id_on UNIV * A \<r>\<e>\<f>\<i>\<n>\<e>\<s> B \<w>.\<r>.\<t> I \<i>\<n> D
 \<Longrightarrow> Id_on UNIV * pairself (fun_upd 1 k) ` A \<r>\<e>\<f>\<i>\<n>\<e>\<s> pairself (fun_upd 1 k) ` B
     \<w>.\<r>.\<t> \<F>_pointwise I \<i>\<n> fun_upd 1 k ` D\<close>
-  for I :: \<open>'c \<Rightarrow> 'b::sep_magma_1 \<Rightarrow> 'a::sep_magma_1 set\<close>
   unfolding Fictional_Forward_Simulation_def
   apply (clarsimp simp add: set_mult_expn Subjection_expn image_iff Image_def subset_iff Bex_def times_fun Id_on_iff)
   subgoal premises prems for r R u v xb xc a b
@@ -342,7 +321,7 @@ lemma \<F>_pointwise_refinement:
       by (metis fun_upd_same prems(8) sep_disj_fun)
     have t2[simp]: \<open>xc k ## b\<close>
       by (metis fun_upd_same prems(9) sep_disj_fun)
-    have \<open>(\<exists>x. (\<exists>ua v. x = ua * v \<and> ua \<in> {u k} \<and> v \<in> I k (r k * xb) \<and> ua ## v) \<and>
+    have \<open>(\<exists>x. (\<exists>ua v. x = ua * v \<and> ua \<in> {u k} \<and> v \<in> \<I> I (r k * xb) \<and> ua ## v) \<and>
      r k ## xb \<and>
      xb \<in> D \<and> (\<exists>a ba aa. x = a * aa \<and> (\<exists>bb. xc k * b = ba * bb \<and> a = ba \<and> (aa, bb) \<in> A \<and> a ## aa \<and> ba ## bb)))\<close>
       by (simp add: prems,
@@ -365,13 +344,14 @@ lemma \<F>_pointwise_refinement:
       qed .
   qed .
 
-(* subsubsection \<open>Pairwise\<close>
+subsubsection \<open>Pairwise\<close>
 
-definition "\<F>_pair I1 I2 = (\<lambda>(x,y). I1 x * I2 y) "
+definition "\<F>_pair I1 I2 = Interp (\<lambda>(x,y). \<I> I1 x * \<I> I2 y) "
 
-lemma \<F>_pair[simp]: "\<F>_pair I1 I2 (x,y) = I1 x * I2 y"
+lemma \<F>_pair_\<I>[simp]: "\<I> (\<F>_pair I1 I2) = (\<lambda>(x,y). \<I> I1 x * \<I> I2 y)"
   for I1 :: "('a::one,'b::sep_monoid) interp"
-  unfolding \<F>_pair_def by (simp add: one_prod_def)
+  unfolding \<F>_pair_def
+  by (rule Interp_inverse) (simp add: Interpretation_def one_prod_def)
 
 notation \<F>_pair (infixl "\<bullet>\<^sub>\<F>" 50)
 
@@ -391,7 +371,7 @@ lemma \<F>_optionwise_\<I>[simp]:
   "\<I> (\<F>_optionwise I) = (\<lambda>x. case x of Some x' \<Rightarrow> Some ` I x' | _ \<Rightarrow> {None})"
   unfolding \<F>_optionwise_def
   by (rule Interp_inverse) (auto simp add: Interpretation_def)
-*)
+
 
 (* subsubsection \<open>Partiality\<close>
 
@@ -411,50 +391,51 @@ lemma partialwise_\<I>[simp]: "\<I> (partialwise I) (Fine x) = { Fine y |y. y \<
 
 subsubsection \<open>Functional Fiction\<close>
 
-definition [simp]: \<open>\<F>_functional \<psi> D x = {y. x = \<psi> y \<and> y \<in> D }\<close>
+definition \<open>\<F>_functional \<psi> D = Interp (\<lambda>x. {y. x = \<psi> y \<and> y \<in> D })\<close>
 
 (* lemma (in kernel_is_1) \<F>_functional_\<I>[simp]:
   \<open>\<I> (\<F>_functional \<psi>) = (\<lambda>x. {y. x = \<psi> y})\<close>
   unfolding \<F>_functional_def
   by (rule Interp_inverse, simp add: Interpretation_def one_set_def set_eq_iff inj_at_1) *)
 
-lemma \<F>_functional_homo_one[simp]:
+lemma \<F>_functional_\<I>[simp]:
   \<open> kernel_is_1 \<psi> D
-\<Longrightarrow> homo_one (\<F>_functional \<psi> D)\<close>
-  unfolding homo_one_def \<F>_functional_def kernel_is_1_def
-  by (clarsimp simp add: set_eq_iff Ball_def; blast)
+\<Longrightarrow> \<I> (\<F>_functional \<psi> D) = (\<lambda>x. {y. x = \<psi> y \<and> y \<in> D })\<close>
+  unfolding \<F>_functional_def kernel_is_1_def
+  by (rule Interp_inverse, auto simp add: Interpretation_def one_set_def set_eq_iff Ball_def)
 
-(*TODO: move this or remove this*)
 lemma map_option_inj_at_1[simp]:
   \<open>kernel_is_1 (map_option f) UNIV\<close>
   unfolding one_option_def kernel_is_1_def
   by (simp add: split_option_all)
 
-lemma (in sep_insertion_monoid) \<F>_functional_projection:
+lemma (in sep_insertion_monoid) \<F>_functional_projection [simp]:
   \<open> S \<subseteq> D
 \<Longrightarrow> refinement_projection (\<F>_functional \<psi> D) (\<psi> ` S) \<subseteq> UNIV * S\<close>
   unfolding refinement_projection_def
   by (clarsimp simp add: subset_iff set_mult_expn eq_commute[where a=\<open>\<psi> _\<close>] sep_insertion; blast)
 
-(*TODO: move this or remove this*)
 lemma kernel_is_1_pointwise[simp,intro!]:
   \<open>kernel_is_1 \<psi> D \<Longrightarrow> kernel_is_1 ((\<circ>) \<psi>) (pointwise_set D)\<close>
   unfolding kernel_is_1_def pointwise_set_def by (simp add: fun_eq_iff)
 
 lemma \<F>_functional_pointwise:
-  \<open>\<F>_functional ((\<circ>) \<psi>) (pointwise_set D) = \<F>_pointwise (\<lambda>_. \<F>_functional \<psi> D)\<close>
-  by (auto simp add: fun_eq_iff set_eq_iff; simp add: pointwise_set_def)
+  \<open> kernel_is_1 \<psi> D
+\<Longrightarrow> \<F>_functional ((\<circ>) \<psi>) (pointwise_set D) = \<F>_pointwise (\<F>_functional \<psi> D)\<close>
+  by (rule interp_eq_I; auto simp add: fun_eq_iff set_eq_iff; simp add: pointwise_set_def)
 
 lemma \<F>_functional_comp:
   \<open> g ` Dg \<subseteq> Df
-\<Longrightarrow> \<F>_functional (f o g) Dg = \<F>_functional g Dg \<Zcomp>\<^sub>\<I> \<F>_functional f Df\<close>
+\<Longrightarrow> kernel_is_1 f Df
+\<Longrightarrow> kernel_is_1 g Dg
+\<Longrightarrow> \<F>_functional (f o g) Dg = \<F>_functional g Dg ;\<^sub>\<I> \<F>_functional f Df\<close>
   by (auto simp add: fun_eq_iff set_eq_iff; blast)
   
 
-(* definition "\<F>_share s = (case s of Share w v \<Rightarrow> if w = 1 then {v} else {})"
+definition "\<F>_share s = (case s of Share w v \<Rightarrow> if w = 1 then {v} else {})"
 
 lemma \<F>_share_\<I>[simp]: "\<F>_share (Share w v) = (if w = 1 then {v} else {})"
-  unfolding \<F>_share_def by simp *)
+  unfolding \<F>_share_def by simp
 
 (* lemma In_ficion_fine [simp]:
   \<open>x \<in> (case some_fine of Fine y \<Rightarrow> f y | Undef \<Rightarrow> {})
@@ -464,8 +445,7 @@ lemma \<F>_share_\<I>[simp]: "\<F>_share (Share w v) = (if w = 1 then {v} else {
 
 subsubsection \<open>Agreement\<close>
 
-(* TODO: check this!!!!
-definition \<open>\<F>_agree = (\<lambda>x. case x of agree x' \<Rightarrow> {x'})\<close> *)
+definition \<open>\<F>_agree = (\<lambda>x. case x of agree x' \<Rightarrow> {x'})\<close>
 
 
 subsection \<open>Refinement of Algebraic Structures\<close>
@@ -480,34 +460,14 @@ lemma refinement_projection:
   apply (clarsimp simp add: set_mult_expn Subjection_expn)
 subgoal for r R u v w *)
 
-definition \<F>_functional_condition
-  where \<open>\<F>_functional_condition D \<longleftrightarrow> (\<forall>r x y. r ## x \<and> r ## y \<and> r \<in> D \<and> x \<in> D \<and> r * x \<in> D \<and> y \<in> D \<longrightarrow> r * y \<in> D)\<close>
-
-lemma \<F>_functional_condition_UNIV[simp]:
-  \<open>\<F>_functional_condition UNIV\<close>
-  unfolding \<F>_functional_condition_def by simp
-
-definition frame_preserving_relation
-  where \<open>frame_preserving_relation R
-    \<longleftrightarrow> (\<forall>a b c d r w. (a,b) \<in> R \<and> (c,d) \<in> R \<and> r * a = w * c \<and> r ## a \<and> r ## b \<and> w ## c
-            \<longrightarrow> r * b = w * d \<and> w ## d)\<close>
-
 context cancl_sep_insertion_monoid begin
-
-lemma \<F>_functional_refinement_complex:
-  \<open> (\<forall>a b. (a,b) \<in> R \<longrightarrow> a \<in> D \<and> b \<in> D)
-\<Longrightarrow> frame_preserving_relation R
-\<Longrightarrow> Sep_Closed D
-\<Longrightarrow> Id_on UNIV * R \<r>\<e>\<f>\<i>\<n>\<e>\<s> pairself \<psi> ` R \<w>.\<r>.\<t> \<F>_functional \<psi> D \<i>\<n> \<psi> ` (Domain R) \<close>
-  unfolding Fictional_Forward_Simulation_def
-  apply (auto simp add: set_mult_expn Subjection_expn sep_insertion Sep_Closed_def image_iff Bex_def)
-  by (smt (z3) frame_preserving_relation_def homo_mult sep_disj_homo_semi sep_disj_multD1 sep_disj_multD2 sep_disj_multI1 sep_disj_multI2 sep_mult_assoc)
 
 lemma \<F>_functional_refinement:
   \<open> a \<in> D \<and> b \<in> D
-\<Longrightarrow> \<F>_functional_condition D
+\<Longrightarrow> (\<forall>r x y. r ## x \<and> r \<in> D \<and> x \<in> D \<and> r * x \<in> D \<and> y \<in> D \<longrightarrow> r * y \<in> D)
+\<Longrightarrow> kernel_is_1 \<psi> D
 \<Longrightarrow> Id_on UNIV * {(a, b)} \<r>\<e>\<f>\<i>\<n>\<e>\<s> pairself \<psi> ` {(a,b)} \<w>.\<r>.\<t> \<F>_functional \<psi> D \<i>\<n> \<psi> ` {a} \<close>
-  unfolding Fictional_Forward_Simulation_def \<F>_functional_condition_def
+  unfolding Fictional_Forward_Simulation_def
   apply (auto simp add: set_mult_expn Subjection_expn sep_insertion)
   apply (metis (no_types, lifting) homo_mult sep_cancel sep_disj_multD1 sep_disj_multD2 sep_disj_multI1 sep_disj_multI2 sep_mult_assoc)
   by (metis sep_cancel sep_disj_homo_semi sep_disj_multD1 sep_disj_multD2 sep_disj_multI1 sep_mult_assoc')
