Phi_Semantics/PhiSem_Mem_C_Base.thy
@@ -1,16 +1,15 @@
 theory PhiSem_Mem_C_Base
-  imports PhiSem_Aggregate_Base
+  imports PhiSem_Aggregate_Base Phi_System.Resource_Template
 begin
 
 section \<open>Semantics\<close>
 
 debt_axiomatization
-        MemObj_Size :: \<open>TY \<Rightarrow> nat\<close>
+        MemObj_Size     :: \<open>TY \<Rightarrow> nat\<close>
     and idx_step_offset :: \<open>TY \<Rightarrow> nat \<Rightarrow> nat\<close>
   where memobj_size_step : \<open>valid_idx_step T i \<Longrightarrow> MemObj_Size (idx_step_type i T) \<le> MemObj_Size T\<close>
     and idx_step_offset_size:
-          \<open>valid_idx_step T i
-                \<Longrightarrow> idx_step_offset T i + MemObj_Size (idx_step_type i T) \<le> MemObj_Size T\<close>
+          \<open>valid_idx_step T i \<Longrightarrow> idx_step_offset T i + MemObj_Size (idx_step_type i T) \<le> MemObj_Size T\<close>
     and idx_step_offset_disj:
           \<open>valid_idx_step T i \<Longrightarrow> valid_idx_step T j \<Longrightarrow>
                 idx_step_offset T i \<le> idx_step_offset T j \<Longrightarrow>
@@ -32,9 +31,9 @@ lemma fold_tail:
 lemma index_offset_upper_bound:
   \<open>valid_index T (base@idx) \<Longrightarrow>
    index_offset T (base@idx) + MemObj_Size (index_type (base@idx) T) \<le> index_offset T base + MemObj_Size (index_type base T)\<close>
-  apply (induct idx arbitrary: base rule: rev_induct;
-         simp del: append_assoc add: append_assoc[symmetric] fold_tail)
-  using idx_step_offset_size by fastforce
+  by (induct idx arbitrary: base rule: rev_induct;
+      simp del: append_assoc add: append_assoc[symmetric] fold_tail;
+      insert idx_step_offset_size, fastforce)
 
 lemmas index_offset_upper_bound_0 = index_offset_upper_bound[where base = "[]", simplified]
 
@@ -55,133 +54,454 @@ lemma index_offset_bound_strict:
 
 section \<open>Fiction\<close>
 
-debt_axiomatization Mapof_Val :: \<open>VAL \<Rightarrow> nat list \<rightharpoonup> VAL\<close>
-  where Mapof_Val_inj: \<open>Va \<in> Well_Type T \<Longrightarrow> Vb \<in> Well_Type T \<Longrightarrow> Mapof_Val Va = Mapof_Val Vb \<Longrightarrow> Va = Vb\<close>
-  and   Mapof_Val_same_dom: \<open>Va \<in> Well_Type T \<Longrightarrow> Vb \<in> Well_Type T \<Longrightarrow> dom (Mapof_Val Va) = dom (Mapof_Val Vb)\<close>
-  and   Mapof_not_1[simp]: \<open>Mapof_Val V \<noteq> 1\<close>
-  and   Mapof_Val_pull_step: \<open>valid_idx_step T i \<Longrightarrow> V \<in> Well_Type T
-                          \<Longrightarrow> pull_map [i] (Mapof_Val V) = Mapof_Val (idx_step_value i V)\<close>
-  and   Mapof_Val_mod_step: \<open>valid_idx_step T i \<Longrightarrow> v \<in> Well_Type T
-                         \<Longrightarrow> Mapof_Val (idx_step_mod_value i f v) = Mapof_Val v ++ push_map [i] (Mapof_Val (f (idx_step_value i v)))\<close>
+debt_axiomatization Map_of_Val :: \<open>VAL \<Rightarrow> nat list \<rightharpoonup> VAL\<close>
+                and Dom_of_TY :: \<open>TY \<Rightarrow> nat list set\<close>
+  where Map_of_Val_inj: \<open>Va \<in> Well_Type T \<Longrightarrow> Vb \<in> Well_Type T \<Longrightarrow> Map_of_Val Va = Map_of_Val Vb \<Longrightarrow> Va = Vb\<close>
+  and   Map_of_Val_dom: \<open>Va \<in> Well_Type T \<Longrightarrow> dom (Map_of_Val Va) = Dom_of_TY T\<close>
+  and   Dom_of_TY_step: \<open>valid_idx_step T i \<Longrightarrow> Dom_of_TY (idx_step_type i T) \<subseteq> Dom_of_TY T\<close>
+  and   Mapof_not_1[simp]: \<open>Map_of_Val V \<noteq> 1\<close>
+  and   Map_of_Val_pull_step: \<open>valid_idx_step T i \<Longrightarrow> V \<in> Well_Type T
+                          \<Longrightarrow> pull_map [i] (Map_of_Val V) = Map_of_Val (idx_step_value i V)\<close>
+  and   Map_of_Val_mod_step: \<open>valid_idx_step T i \<Longrightarrow> v \<in> Well_Type T
+                         \<Longrightarrow> Map_of_Val (idx_step_mod_value i f v) = Map_of_Val v ++ push_map [i] (Map_of_Val (f (idx_step_value i v)))\<close>
 
-lemma Mapof_Val_pull:
-  \<open>valid_index T idx \<Longrightarrow> V \<in> Well_Type T \<Longrightarrow> pull_map idx (Mapof_Val V) = Mapof_Val (index_value idx V)\<close>
-  apply (induct idx arbitrary: V T; simp)
-  using Mapof_Val_pull_step
-  by (metis idx_step_value_welltyp pull_map_cons)
+lemma Map_of_Val_pull:
+  \<open>valid_index T idx \<Longrightarrow> V \<in> Well_Type T \<Longrightarrow> pull_map idx (Map_of_Val V) = Map_of_Val (index_value idx V)\<close>
+  by (induct idx arbitrary: V T; simp; metis Map_of_Val_pull_step idx_step_value_welltyp pull_map_cons)
 
+lemma Dom_of_TY:
+  \<open>valid_index T idx \<Longrightarrow> Dom_of_TY (index_type idx T) \<subseteq> Dom_of_TY T\<close>
+  by (induct idx arbitrary: T; simp; meson Dom_of_TY_step dual_order.trans)
+
+(* depreciated
 lemma total_Mapof_disjoint:
    \<open>g ## (push_map idx (to_share \<circ> h))
 \<Longrightarrow> to_share \<circ> f = g * (push_map idx (to_share \<circ> h))
 \<Longrightarrow> dom g \<inter> dom (push_map idx (to_share \<circ> h)) = {}\<close>
-  using to_share_total_disjoint push_map_to_share by metis
+  using to_share_total_disjoint push_map_to_share by metis *)
 
 lemma map_add_subsumed_dom:
   \<open>dom f \<subseteq> dom g \<Longrightarrow> f ++ g = g\<close>
   unfolding map_add_def dom_def subset_eq fun_eq_iff apply simp
   by (metis option.case_eq_if option.collapse option.simps(3))
 
-lemma Mapof_Val_mod:
+lemma Map_of_Val_mod:
   \<open> valid_index T idx
 \<Longrightarrow> v \<in> Well_Type T
 \<Longrightarrow> u \<in> Well_Type (index_type idx T)
-\<Longrightarrow> Mapof_Val (index_mod_value idx (\<lambda>_. u) v) = Mapof_Val v ++ push_map idx (Mapof_Val u)\<close>
+\<Longrightarrow> Map_of_Val (index_mod_value idx (\<lambda>_. u) v) = Map_of_Val v ++ push_map idx (Map_of_Val u)\<close>
   apply (induct idx arbitrary: u v T; simp)
-  using Mapof_Val_same_dom map_add_subsumed_dom apply (metis order_refl)
-  by clarify (simp add: idx_step_value_welltyp Mapof_Val_mod_step  push_map_distrib_map_add
-                        Mapof_Val_pull_step[symmetric] push_pull_map map_add_subsumed2
+  using Map_of_Val_dom map_add_subsumed_dom apply (metis order_refl)
+  by clarify (simp add: idx_step_value_welltyp Map_of_Val_mod_step  push_map_distrib_map_add
+                        Map_of_Val_pull_step[symmetric] push_pull_map map_add_subsumed2
                         push_map_push_map)
 
-lemma Mapof_Val_modify_fiction:
+(* lemma Map_of_Val_modify_fiction:
    \<open>valid_index T idx
 \<Longrightarrow> v \<in> Well_Type T
 \<Longrightarrow> u \<in> Well_Type (index_type idx T)
 \<Longrightarrow> u'\<in> Well_Type (index_type idx T)
-\<Longrightarrow> g ## (push_map idx (to_share \<circ> Mapof_Val u))
-\<Longrightarrow> to_share \<circ> (Mapof_Val v) = g * (push_map idx (to_share \<circ> Mapof_Val u))
-\<Longrightarrow> to_share \<circ> (Mapof_Val (index_mod_value idx (\<lambda>_. u') v)) = g * (push_map idx (to_share \<circ> Mapof_Val u'))\<close>
-  apply (simp add: Mapof_Val_mod to_share_funcomp_map_add push_map_to_share
+\<Longrightarrow> g ## (push_map idx (to_share \<circ> Map_of_Val u))
+\<Longrightarrow> to_share \<circ> (Map_of_Val v) = g * (push_map idx (to_share \<circ> Map_of_Val u))
+\<Longrightarrow> to_share \<circ> (Map_of_Val (index_mod_value idx (\<lambda>_. u') v)) = g * (push_map idx (to_share \<circ> Map_of_Val u'))\<close>
+  apply (simp add: Map_of_Val_mod to_share_funcomp_map_add push_map_to_share
       times_fun_map_add_right total_Mapof_disjoint[simplified push_map_to_share]
-      Mapof_Val_same_dom push_map_dom_eq)
+      Map_of_Val_same_dom push_map_dom_eq)
   subgoal premises prems proof -
-    have \<open>dom g \<inter> dom (to_share \<circ> push_map idx (Mapof_Val u)) = {}\<close>
+    have \<open>dom g \<inter> dom (to_share \<circ> push_map idx (Map_of_Val u)) = {}\<close>
       using prems to_share_total_disjoint by blast
     moreover have t1:
-      \<open>dom (to_share \<circ> push_map idx (Mapof_Val u)) = dom (to_share \<circ> push_map idx (Mapof_Val u'))\<close>
-      using prems by (metis Mapof_Val_same_dom dom_map_option_comp push_map_dom_eq)
-    ultimately have \<open>dom g \<inter> dom (to_share \<circ> push_map idx (Mapof_Val u')) = {}\<close> by metis
+      \<open>dom (to_share \<circ> push_map idx (Map_of_Val u)) = dom (to_share \<circ> push_map idx (Map_of_Val u'))\<close>
+      using prems by (metis Map_of_Val_same_dom dom_map_option_comp push_map_dom_eq)
+    ultimately have \<open>dom g \<inter> dom (to_share \<circ> push_map idx (Map_of_Val u')) = {}\<close> by metis
     note [simp] = times_fun_map_add_right[OF this]
     show ?thesis by simp (metis t1 map_add_subsumed_dom order_eq_refl)
   qed
   done
 (* lemma pull_map_share_Mapof_not_eq_1[simp]:
-  \<open>valid_index (Typeof v) idx \<Longrightarrow> pull_map idx (share n (to_share \<circ> Mapof_Val v)) = 1 \<longleftrightarrow> n = 0\<close>
-  by (cases \<open>n = 0\<close>; simp add: pull_map_share pull_map_to_share Mapof_Val_pull)
-*)
+  \<open>valid_index (Typeof v) idx \<Longrightarrow> pull_map idx (share n (to_share \<circ> Map_of_Val v)) = 1 \<longleftrightarrow> n = 0\<close>
+  by (cases \<open>n = 0\<close>; simp add: pull_map_share pull_map_to_share Map_of_Val_pull)
+*)*)
 
-
+(* depreciated
 lemma map_add_restrict_itself [simp]: \<open>(f ++ g) |` dom g = g\<close>
   unfolding fun_eq_iff restrict_map_def map_add_def
   by (simp add: domIff option.case_eq_if)
 
-lemma Mapof_Val_inj_plus:
-  \<open>Va \<in> Well_Type T \<Longrightarrow> Vb \<in> Well_Type T \<Longrightarrow> f ++ Mapof_Val Va = f ++ Mapof_Val Vb \<Longrightarrow> Va = Vb\<close>
-proof (rule Mapof_Val_inj, assumption)
+lemma Map_of_Val_inj_plus:
+  \<open>Va \<in> Well_Type T \<Longrightarrow> Vb \<in> Well_Type T \<Longrightarrow> f ++ Map_of_Val Va = f ++ Map_of_Val Vb \<Longrightarrow> Va = Vb\<close>
+proof (rule Map_of_Val_inj, assumption)
   assume tyA: \<open>Va \<in> Well_Type T\<close>
      and tyB: \<open>Vb \<in> Well_Type T\<close>
-     and feq: \<open>f ++ Mapof_Val Va = f ++ Mapof_Val Vb\<close>
-  then have \<open>(f ++ Mapof_Val Va) |` dom (Mapof_Val Va) = (f ++ Mapof_Val Vb) |` dom (Mapof_Val Vb)\<close>
-    using Mapof_Val_same_dom by metis 
+     and feq: \<open>f ++ Map_of_Val Va = f ++ Map_of_Val Vb\<close>
+  then have \<open>(f ++ Map_of_Val Va) |` dom (Map_of_Val Va) = (f ++ Map_of_Val Vb) |` dom (Map_of_Val Vb)\<close>
+    using Map_of_Val_dom by metis 
   note this [simplified]
-  then show \<open>Mapof_Val Va = Mapof_Val Vb\<close> .
+  then show \<open>Map_of_Val Va = Map_of_Val Vb\<close> .
 qed
 
-definition \<open>Valof_Map TY M = (@V. (\<exists>f. f ++ Mapof_Val V = M) \<and> V \<in> Well_Type TY)\<close>
+definition \<open>Val_of_Map TY M = (@V. (\<exists>f. f ++ Map_of_Val V = M) \<and> V \<in> Well_Type TY)\<close>
 
-lemma Valof_Map_append[simp]:
-  \<open>v \<in> Well_Type T \<Longrightarrow> Valof_Map T (f ++ Mapof_Val v) = v\<close>
-  unfolding Valof_Map_def
-  using someI[where P=\<open>\<lambda>V. (\<exists>fa. fa ++ Mapof_Val V = f ++ Mapof_Val v) \<and> V \<in> Well_Type T\<close> and x=v, simplified]
-        Mapof_Val_inj_plus
-  by (metis (no_types, lifting) Mapof_Val_same_dom map_add_restrict_itself) 
+lemma Val_of_Map_append[simp]:
+  \<open>v \<in> Well_Type T \<Longrightarrow> Val_of_Map T (f ++ Map_of_Val v) = v\<close>
+  unfolding Val_of_Map_def
+  using someI[where P=\<open>\<lambda>V. (\<exists>fa. fa ++ Map_of_Val V = f ++ Map_of_Val v) \<and> V \<in> Well_Type T\<close> and x=v, simplified]
+        Map_of_Val_inj_plus
+  by (metis (no_types, lifting) Map_of_Val_dom map_add_restrict_itself) 
 
-lemmas Valof_Map[simp] = Valof_Map_append[where f = \<open>Map.empty\<close>, simplified]
+lemmas Val_of_Map[simp] = Val_of_Map_append[where f = \<open>Map.empty\<close>, simplified] *)
 
+definition Map_of_Val_ins
+  where \<open>Map_of_Val_ins = ((o) (map_option nosep))
+                            o (\<lambda>V. (case V of Some V' \<Rightarrow> Map_of_Val V' | None \<Rightarrow> 1))
+                            o map_option nosep.dest\<close>
+definition Map_of_Val_ins_dom
+  where \<open>Map_of_Val_ins_dom TY = {x. pred_option (\<lambda>x'. nosep.dest x' \<in> Well_Type TY) x}\<close>
 
-lemma
-  \<open> perm_ins_homo' f
-\<Longrightarrow> perm_ins_homo' (\<lambda>v. f o Mapof_Val v)\<close>
+lemma Map_of_Val_ins_eval[simp]:
+  \<open>Map_of_Val_ins (Some (nosep u)) = (map_option nosep) o Map_of_Val u\<close>
+  \<open>Map_of_Val_ins None = 1\<close>
+  unfolding Map_of_Val_ins_def by simp+
 
-  term \<open>(\<lambda>v. f o Mapof_Val v)\<close>
-  term Mapof_Val
-  term \<open>((o) to_share) o Mapof_Val\<close>
+lemma Map_of_Val_ins_dom_eval[simp]:
+  \<open>Some (nosep u) \<in> Map_of_Val_ins_dom TY \<longleftrightarrow> u \<in> Well_Type TY\<close>
+  unfolding Map_of_Val_ins_dom_def by simp
 
-
-
-
-
-definition \<open>fic_val_to_share_map TY =
-      Interp (\<lambda>m. if m = 1 then {None} else {Some v |v. v \<in> Well_Type TY \<and> to_share o Mapof_Val v = m})\<close>
-
-lemma fic_val_to_share_map[simp]:
-  \<open>\<I> (fic_val_to_share_map TY) = (\<lambda>m. if m = 1 then {None} else {Some v |v. v \<in> Well_Type TY \<and> to_share o Mapof_Val v = m})\<close>
-  unfolding fic_val_to_share_map_def by (rule Interp_inverse) (simp add: Interpretation_def one_set_def)
-
-
-paragraph \<open>Basic fictions for resource elements\<close>
+lemma \<F>_functional_condition_Map_of_Val_ins_dom:
+  \<open>\<F>_functional_condition (Map_of_Val_ins_dom TY)\<close>
+  unfolding \<F>_functional_condition_def Map_of_Val_ins_dom_def
+  by (clarsimp; case_tac r; case_tac x; simp)
 
 
+interpretation Map_of_Val_ins: cancl_sep_insertion_monoid \<open>Map_of_Val_ins\<close> \<open>Map_of_Val_ins_dom TY\<close>
+  apply (standard; clarsimp simp add: Map_of_Val_ins_def split_nosep_meta_all
+                                      Map_of_Val_ins_dom_def
+                            split: option.split)
 
-definition "share_mem' = 
-              fiction.pointwise' (\<lambda>seg.  (share_val_fiction (segidx.layout seg)))"
+  apply (auto simp add: fun_eq_iff split_option_ex times_fun 
+                                  sep_disj_fun_def split_nosep_meta_all
+                        split: option.split)[1]
+  using Mapof_not_1 apply fastforce
+  apply (metis Map_of_Val_dom domIff option.map_disc_iff times_option(2))
+  subgoal premises prems for a x x' proof -
+    have t1: \<open>a x = 1\<close> for x
+      by (metis Map_of_Val_dom domIff one_option_def option.map_disc_iff prems(1) prems(2) prems(3) prems(4) times_option(2))
+    have t2: \<open>map_option nosep o Map_of_Val x = map_option nosep o Map_of_Val x'\<close>
+      using prems(4) t1 by auto
+    show ?thesis
+      by (metis (mono_tags, lifting) Map_of_Val_inj fun.inj_map_strong nosep.inject option.inj_map_strong prems(2) prems(3) t2) 
+  qed .
 
-definition "share_mem = fiction_mem (fiction.defined (
-              fiction.pointwise' (\<lambda>seg. fiction.fine (share_val_fiction (segidx.layout seg)))))"
+lemma map_tree_refinement_modify:
+  \<open> dom a = dom b \<and> dom b \<subseteq> D
+\<Longrightarrow> (\<And>r. r ## push_map idx a \<and> r ## push_map idx b \<and> r * push_map idx a \<in> S \<Longrightarrow> r * push_map idx b \<in> S)
+\<Longrightarrow> Id_on UNIV * ({(a, a ++ push_map idx b)} \<s>\<u>\<b>\<j> a. dom a = D)
+    \<r>\<e>\<f>\<i>\<n>\<e>\<s> { (push_map idx a, push_map idx b)}
+    \<w>.\<r>.\<t> \<F>_functional id S
+    \<i>\<n> { push_map idx a }\<close>
+  for a :: \<open>'a list \<Rightarrow> VAL nosep option\<close>
+  unfolding Fictional_Forward_Simulation_def the_subtree_def
+  apply (clarsimp simp add: Subjection_expn set_mult_expn ExSet_expn)
+  subgoal premises prems for r R a' u x
+  proof -
+    have t1: \<open>dom x \<inter> dom (idx \<^enum>\<^sub>m b) = {}\<close>
+      using disjoint_iff prems(10) sep_disj_partial_map_disjoint by fastforce
+    have t2: \<open>dom r \<inter> dom (idx \<^enum>\<^sub>m b) = {}\<close>
+      by (metis prems(2) prems(4) push_map_dom_eq sep_disj_partial_map_disjoint)
+    have t3: \<open>dom u \<inter> dom (idx \<^enum>\<^sub>m b) = {}\<close>
+      by (metis prems(12) prems(2) push_map_dom_eq sep_disj_partial_map_disjoint)
+    have t4: \<open>u ## idx \<^enum>\<^sub>m b\<close>
+      using sep_disj_partial_map_disjoint t3 by blast
+    have t5: \<open>r ## idx \<^enum>\<^sub>m b\<close>
+      using sep_disj_partial_map_disjoint t2 by blast
+    have t6: \<open>dom x \<inter> dom a' = {}\<close>
+      by (meson prems(9) sep_disj_partial_map_disjoint)
+    show ?thesis
+      apply (simp add: t5, rule exI[where x=u], simp add: t4 prems)
+      by (smt (verit, best) map_add_subsumed_dom mult.left_commute prems(1) prems(2) prems(4) prems(6) prems(8) push_map_distrib_map_add t1 t2 t3 t5 times_fun_map_add_right verit_comp_simplify1(2))
+  qed .
 
-lemma share_mem_def':
-  \<open>share_mem = fiction_mem (fiction.defined share_mem')\<close>
-  unfolding share_mem_def share_mem'_def ..
+lemma fiction_Map_of_Val_ins_comp_id_simp:
+  \<open>(\<F>_functional Map_of_Val_ins (Map_of_Val_ins_dom TY) \<Zcomp>\<^sub>\<I>
+    \<F>_functional id (Map_of_Val_ins ` Map_of_Val_ins_dom TY))
+  = \<F>_functional Map_of_Val_ins (Map_of_Val_ins_dom TY)\<close>
+  by (rule \<F>_functional_comp[where f=id, simplified, symmetric]; clarsimp)
+
+lemma val_map_eq_index_value_eq:
+  \<open>valid_index TY idx \<Longrightarrow>
+    u_idx \<in> Well_Type (index_type idx TY) \<Longrightarrow>
+    v \<in> Well_Type TY \<Longrightarrow>
+    map_option nosep \<circ> Map_of_Val v = u * idx \<^enum>\<^sub>m (map_option nosep \<circ> Map_of_Val u_idx) \<Longrightarrow>
+    u ## idx \<^enum>\<^sub>m (map_option nosep \<circ> Map_of_Val u_idx) \<Longrightarrow>
+    index_value idx v = u_idx \<close>
+  subgoal premises prems proof -
+    have t1: \<open>dom (pull_map idx (Map_of_Val v)) = Dom_of_TY (index_type idx TY)\<close>
+      using Map_of_Val_dom Map_of_Val_pull index_value_welltyp prems(1) prems(3) by auto
+    have t2: \<open>dom (pull_map idx (Map_of_Val v)) =
+              dom (pull_map idx u) \<union> dom (Map_of_Val u_idx)\<close>
+      by (metis dom1_dom dom1_mult dom_map_option_comp map_option_homo_one prems(4) prems(5) pull_map_funcomp pull_map_homo_mult pull_map_sep_disj pull_push_map)
+    have t3: \<open>dom (pull_map idx u) \<inter> dom (Map_of_Val u_idx) = {}\<close>
+      by (metis dom1_dom dom_map_option_comp prems(5) pull_map_sep_disj pull_push_map sep_disj_dom1_disj_disjoint)
+    have t4: \<open>dom (Map_of_Val u_idx) = Dom_of_TY (index_type idx TY)\<close>
+      using Map_of_Val_dom prems(2) by force
+    have t5: \<open>pull_map idx u = 1\<close>
+      using t1 t2 t3 t4 by fastforce
+    then have \<open>pull_map idx (map_option nosep \<circ> Map_of_Val v) = (map_option nosep \<circ> Map_of_Val u_idx)\<close>
+      by (simp add: prems(4) pull_map_homo_mult)
+    then have \<open>pull_map idx (Map_of_Val v) = Map_of_Val u_idx\<close>
+      by (smt (verit) fun.inj_map_strong map_option_homo_one nosep.inject option.inj_map_strong pull_map_funcomp)
+    then show ?thesis
+      by (metis Map_of_Val_inj Map_of_Val_pull index_value_welltyp prems(1) prems(2) prems(3))
+  qed .
+
+lemma val_map_mod_index_value:
+  \<open> valid_index TY idx \<Longrightarrow>
+    x \<in> Well_Type TY \<Longrightarrow>
+    u \<in> Well_Type (index_type idx TY) \<Longrightarrow>
+    v \<in> Well_Type (index_type idx TY) \<Longrightarrow>
+    r ## idx \<^enum>\<^sub>m (map_option nosep \<circ> Map_of_Val u) \<Longrightarrow>
+    r ## idx \<^enum>\<^sub>m (map_option nosep \<circ> Map_of_Val v) \<Longrightarrow>
+    r * idx \<^enum>\<^sub>m (map_option nosep \<circ> Map_of_Val u) = map_option nosep \<circ> Map_of_Val x \<Longrightarrow>
+    r * idx \<^enum>\<^sub>m (map_option nosep \<circ> Map_of_Val v) = map_option nosep \<circ> Map_of_Val (index_mod_value idx (\<lambda>_. v) x)\<close>
+  by (simp add: Map_of_Val_mod map_option_funcomp_map_add,
+      smt (verit) Map_of_Val_dom dom_map_option_comp map_add_subsumed_dom map_le_implies_dom_le map_option_homo_one pull_push_map push_map_dom_eq push_map_homo push_pull_map sep_disj_partial_map_disjoint times_fun_map_add_right)
+
+lemma val_map_mod_index_value_projection:
+  \<open> valid_index TY idx \<Longrightarrow>
+    u_idx \<in> Well_Type (index_type idx TY) \<Longrightarrow>
+    refinement_projection (\<F>_functional id (Map_of_Val_ins ` Map_of_Val_ins_dom TY)) {idx \<^enum>\<^sub>m (map_option nosep \<circ> Map_of_Val u_idx)}
+    \<subseteq> UNIV * Map_of_Val_ins ` Some ` nosep ` {a. index_value idx a = u_idx \<and> a \<in> Well_Type TY}\<close>
+  apply (clarsimp simp add: image_iff set_mult_expn refinement_projection_def
+                            Map_of_Val_ins_dom_def Map_of_Val_ins_def;
+         case_tac xb; simp add: split_nosep_meta_all)
+  apply (smt (verit, best) Mapof_not_1 dom_1 dom_eq_empty_conv dom_map_option_comp)
+  by (metis mult.commute mult_1_class.mult_1_right sep_magma_1_right val_map_eq_index_value_eq)
+
+lemma fiction_Map_of_Val_ins_projection:
+  \<open> valid_index TY idx
+\<Longrightarrow> u_idx \<in> Well_Type (index_type idx TY)
+\<Longrightarrow> refinement_projection (\<F>_functional Map_of_Val_ins (Map_of_Val_ins_dom TY))
+                          {idx \<^enum>\<^sub>m (map_option nosep \<circ> Map_of_Val u_idx)}
+      \<subseteq> UNIV * Some ` nosep ` {a. index_value idx a = u_idx \<and> a \<in> Well_Type TY }\<close>
+  apply (subst fiction_Map_of_Val_ins_comp_id_simp[symmetric])
+  apply (rule refinement_projections_stepwise_UNIV_paired)
+  apply (rule Map_of_Val_ins.\<F>_functional_projection)
+  apply (clarsimp)
+  by (insert val_map_mod_index_value_projection)
+
+lemma fiction_Map_of_Val_ins_projection':
+  \<open> valid_index TY idx
+\<Longrightarrow> u_idx \<in> Well_Type (index_type idx TY)
+\<Longrightarrow> refinement_projection (\<F>_functional Map_of_Val_ins (Map_of_Val_ins_dom TY))
+                          {idx \<^enum>\<^sub>m (map_option nosep \<circ> Map_of_Val u_idx)}
+      \<subseteq> UNIV * Some ` nosep ` {a. index_value idx a = u_idx }\<close>
+  subgoal premises prems proof -
+    have \<open> UNIV * Some ` nosep ` {a. index_value idx a = u_idx \<and> a \<in> Well_Type TY }
+        \<subseteq> UNIV * Some ` nosep ` {a. index_value idx a = u_idx }\<close>
+      by (simp add: Collect_mono_iff image_mono)
+    then show ?thesis
+      using fiction_Map_of_Val_ins_projection prems(1) prems(2) by blast
+  qed .
+
+lemma fiction_Map_of_Val_ins_refinement:
+  \<open> valid_index TY idx
+\<Longrightarrow> v \<in> Well_Type (index_type idx TY)
+\<Longrightarrow> u_idx \<in> Well_Type (index_type idx TY)
+\<Longrightarrow> Id_on UNIV * ({(Some u, (Some o map_nosep (index_mod_value idx (\<lambda>_. v))) u)}
+                    \<s>\<u>\<b>\<j> u. u \<in> nosep ` {a. index_value idx a = u_idx}
+                      \<and> u \<in> nosep ` Well_Type TY)
+    \<r>\<e>\<f>\<i>\<n>\<e>\<s> {(idx \<^enum>\<^sub>m (map_option nosep \<circ> Map_of_Val u_idx),
+            idx \<^enum>\<^sub>m (map_option nosep \<circ> Map_of_Val v))}
+    \<w>.\<r>.\<t> \<F>_functional Map_of_Val_ins (Map_of_Val_ins_dom TY)
+    \<i>\<n> {idx \<^enum>\<^sub>m (map_option nosep \<circ> Map_of_Val u_idx)}\<close>
+  apply (subst fiction_Map_of_Val_ins_comp_id_simp[symmetric])
+  apply (rule sep_refinement_stepwise[
+            OF refinement_frame[where R = UNIV, OF Map_of_Val_ins.\<F>_functional_refinement_complex[simplified]]])
+  apply (simp add: ExSet_expn Subjection_expn split_nosep_ex inj_image_mem_iff split_option_all
+                   split_nosep_all index_mod_value_welltyp)
+  apply (simp add: frame_preserving_relation_def split_option_all split_nosep_all
+                   ExSet_expn Subjection_expn)
+  apply (simp add: Sep_Closed_def)
+  subgoal premises prems proof -
+    have t1: \<open>B \<subseteq> B' \<Longrightarrow> A * B \<subseteq> A * B'\<close> for A B B'
+      by (clarsimp simp add: subset_iff set_mult_expn; blast)
+    have \<open>pairself Map_of_Val_ins `
+            ({(Some u, (Some \<circ> map_nosep (index_mod_value idx (\<lambda>_. v))) u)} \<s>\<u>\<b>\<j> u.
+             u \<in> nosep ` {a. index_value idx a = u_idx} \<and> u \<in> nosep ` Well_Type TY)
+        \<subseteq> ({(a, a ++ (idx \<^enum>\<^sub>m (map_option nosep \<circ> Map_of_Val v)))} \<s>\<u>\<b>\<j> a. dom a = Dom_of_TY TY)\<close>
+      apply (clarsimp simp add: set_eq_iff ExSet_image Subjection_image;
+             auto simp add: ExSet_expn Subjection_expn split_nosep_ex inj_image_mem_iff)
+      apply (metis Map_of_Val_mod map_option_funcomp_map_add map_option_homo_one prems(1) prems(2) push_map_homo)
+      using Map_of_Val_dom apply blast
+      using Map_of_Val_dom by blast
+    note t2 = this[THEN t1, THEN refinement_sub_fun]
+    have t3: \<open>dom (Map_of_Val v) = Dom_of_TY (index_type idx TY)\<close>
+      using Map_of_Val_dom prems(2) by force
+    have t4: \<open>idx \<^enum>\<^sub>m (map_option nosep \<circ> Map_of_Val u_idx) \<noteq> 1\<close>
+      by (smt (verit) Mapof_not_1 dom_1 dom_eq_empty_conv dom_map_option_comp push_map_eq_1)
+    then have t5: \<open> r * idx \<^enum>\<^sub>m (map_option nosep \<circ> Map_of_Val u_idx) \<noteq> 1\<close> for r
+      by (metis (no_types, opaque_lifting) dom1_disjoint_sep_disj dom1_dom dom_eq_empty_conv empty_subsetI inf.orderE one_partial_map sep_no_inverse times_fun_def times_option_none)
+    show ?thesis
+      apply (rule t2)
+      apply (rule map_tree_refinement_modify)
+      apply (simp add: Dom_of_TY Map_of_Val_dom prems(1) prems(3) t3)
+      apply (simp add: Map_of_Val_ins_def Map_of_Val_ins_dom_def image_iff split_option_ex
+                       split_nosep_ex split_nosep_meta_all split_nosep_all t5)
+      by (metis index_mod_value_welltyp prems(1) prems(2) prems(3) val_map_mod_index_value)
+  qed
+  subgoal premises prems proof -
+    have t1: \<open> Domain ({(a u, b u)} \<s>\<u>\<b>\<j> u. P u) = { a u |u. P u }\<close> for a b P
+      unfolding set_eq_iff Domain_unfold by (clarsimp simp add: ExSet_expn Subjection_expn)
+    have t2: \<open>{Some u |u. u \<in> nosep ` {a. index_value idx a = u_idx} \<and> u \<in> nosep ` Well_Type TY}
+                = Some ` nosep ` {a. index_value idx a = u_idx \<and> a \<in> Well_Type TY}\<close>
+      by (clarsimp simp add: set_eq_iff image_iff Bex_def; blast)
+
+    show ?thesis
+      by (subst t1, subst t2, rule val_map_mod_index_value_projection, insert prems(1) prems(3))
+  qed .
 
 
+lemma fiction_Map_of_Val_perm_partial_refinement:
+  \<open> valid_index TY idx
+\<Longrightarrow> v \<in> Well_Type (index_type idx TY)
+\<Longrightarrow> u_idx \<in> Well_Type (index_type idx TY)
+\<Longrightarrow> Id_on UNIV * ({(Some u, (Some o map_nosep (index_mod_value idx (\<lambda>_. v))) u)}
+                    \<s>\<u>\<b>\<j> u. u \<in> nosep ` {a. index_value idx a = u_idx}
+                      \<and> u \<in> nosep ` Well_Type TY)
+    \<r>\<e>\<f>\<i>\<n>\<e>\<s> {(to_share o idx \<^enum>\<^sub>m (map_option nosep \<circ> Map_of_Val u_idx),
+            to_share o idx \<^enum>\<^sub>m (map_option nosep \<circ> Map_of_Val v))}
+    \<w>.\<r>.\<t> \<F>_functional((\<circ>) to_share \<circ> Map_of_Val_ins) (Map_of_Val_ins_dom TY)
+    \<i>\<n> {to_share o idx \<^enum>\<^sub>m (map_option nosep \<circ> Map_of_Val u_idx)}\<close>
+  unfolding \<F>_functional_comp[where f=\<open>(\<circ>) to_share\<close> and Df=\<open>UNIV\<close>, simplified]
+  by (rule sep_refinement_stepwise,
+      rule refinement_frame[OF fiction_Map_of_Val_ins_refinement],
+      assumption,
+      assumption,
+      assumption,
+      rule pointwise_to_share.\<F>_functional_refinement[simplified, simplified pointwise_set_UNIV],
+      simp,
+      simp,
+      rule pointwise_to_share.\<F>_functional_projection[
+        where S=\<open>{idx \<^enum>\<^sub>m (map_option nosep \<circ> Map_of_Val u_idx)}\<close>, simplified, simplified pointwise_set_UNIV],
+      simp)
+
+lemma fiction_Map_of_Val_ins_perm_projection:
+  \<open> valid_index TY idx
+\<Longrightarrow> u_idx \<in> Well_Type (index_type idx TY)
+\<Longrightarrow> refinement_projection (\<F>_functional ((\<circ>) to_share o Map_of_Val_ins) (Map_of_Val_ins_dom TY))
+                          { to_share o idx \<^enum>\<^sub>m (map_option nosep \<circ> Map_of_Val u_idx) }
+      \<subseteq> UNIV * Some ` nosep ` {a. index_value idx a = u_idx }\<close>
+  unfolding \<F>_functional_comp[where f=\<open>(\<circ>) to_share\<close> and Df=\<open>UNIV\<close>, simplified]
+  by (rule refinement_projections_stepwise_UNIV_paired,
+      rule fiction_Map_of_Val_ins_projection',
+      assumption,
+      assumption,
+      rule pointwise_to_share.\<F>_functional_projection[
+        where S=\<open>{idx \<^enum>\<^sub>m (map_option nosep \<circ> Map_of_Val u_idx)}\<close>, simplified, simplified pointwise_set_UNIV],
+      simp)
+
+locale pointer_mem_resource =
+  partial_map_resource Res \<open>\<lambda>blk. nosep ` Well_Type (typ_of_blk blk)\<close>
+  for Res :: "('blk \<Rightarrow> VAL nosep option) resource_entry"
+  and typ_of_blk :: \<open>'blk \<Rightarrow> TY\<close>
+
+locale perm_pointer_mem_fiction =
+  pointwise_base_fiction_for_partial_mapping_resource
+      Res \<open>\<lambda>blk. \<F>_functional ((\<circ>) to_share \<circ> Map_of_Val_ins) (Map_of_Val_ins_dom (typ_of_blk blk))\<close>
+      Fic \<open>\<lambda>blk. nosep ` Well_Type (typ_of_blk blk)\<close>
+  for Res :: "('blk \<Rightarrow> VAL nosep option) resource_entry"
+  and Fic :: "('blk \<Rightarrow> nat list \<Rightarrow> VAL nosep share option) fiction_entry"
+  and typ_of_blk :: \<open>'blk \<Rightarrow> TY\<close>
+begin
+
+sublocale pointer_mem_resource Res typ_of_blk ..
+
+lemma getter_rule:
+  \<open> valid_index (typ_of_blk blk) idx
+\<Longrightarrow> u_idx \<in> Well_Type (index_type idx (typ_of_blk blk))
+\<Longrightarrow> \<p>\<r>\<o>\<c> R.\<phi>R_get_res_entry' blk \<lbrace> 1(blk := to_share \<circ> idx \<^enum>\<^sub>m (map_option nosep \<circ> Map_of_Val u_idx)) \<Ztypecolon> \<phi> Identity \<longmapsto>
+      \<lambda>ret. 1(blk := to_share \<circ> idx \<^enum>\<^sub>m (map_option nosep \<circ> Map_of_Val u_idx)) \<Ztypecolon> \<phi> Identity
+          \<s>\<u>\<b>\<j> x. ret = \<phi>arg (nosep x) \<and> x \<in> Well_Type (typ_of_blk blk) \<and> x \<in> {a. index_value idx a = u_idx} \<rbrace>\<close>
+  by (rule "_getter_rule_2_"[OF fiction_Map_of_Val_ins_perm_projection,
+                                simplified split_nosep_ExSet inj_image_mem_iff inj_nosep])
+
+lemma allocate_rule:
+  \<open> (\<And>r. finite (dom r) \<Longrightarrow> \<exists>blk. blk \<notin> dom r \<and> typ_of_blk blk = TY)
+\<Longrightarrow> v \<in> Well_Type TY
+\<Longrightarrow> \<p>\<r>\<o>\<c> R.\<phi>R_allocate_res_entry' (\<lambda>blk. typ_of_blk blk = TY) (Some (nosep v))
+      \<lbrace> Void \<longmapsto> \<lambda>ret. 1(blk := to_share \<circ> (map_option nosep \<circ> Map_of_Val v)) \<Ztypecolon> \<phi> Identity \<s>\<u>\<b>\<j> blk. ret = \<phi>arg blk \<and> typ_of_blk blk = TY  \<rbrace> \<close>
+  subgoal premises prems proof-
+
+  note pointwise_set_UNIV[simp] \<F>_functional_condition_Map_of_Val_ins_dom[simp]
+
+  show ?thesis
+  by (rule "__allocate_rule_3__",
+      unfold \<F>_functional_comp[where f=\<open>(\<circ>) to_share\<close> and Df=\<open>UNIV\<close>, simplified, simp]
+             one_option_def,
+      rule sep_refinement_stepwise[
+                  OF refinement_frame[OF Map_of_Val_ins.\<F>_functional_refinement[simplified]]
+                     pointwise_to_share.\<F>_functional_refinement
+                     pointwise_to_share.\<F>_functional_projection,
+                  where a4=\<open>None\<close> and b4=\<open>Some (nosep u)\<close> for u,
+                  simplified],
+      simp add: Map_of_Val_ins_dom_def prems(2),
+      simp add: R.in_invariant inj_image_mem_iff prems(2),
+      clarsimp simp add: R.in_invariant Ball_def dom1_dom, metis dom_map_option_comp prems(1))
+qed .
+
+lemma setter_rule:
+  \<open> valid_index (typ_of_blk blk) idx
+\<Longrightarrow> v \<in> Well_Type (index_type idx (typ_of_blk blk))
+\<Longrightarrow> u_idx \<in> Well_Type (index_type idx (typ_of_blk blk))
+\<Longrightarrow> \<p>\<r>\<o>\<c> R.\<phi>R_set_res' (map_fun_at blk (Some \<circ> map_nosep (index_mod_value idx (\<lambda>_. v)) \<circ> the))
+      \<lbrace> 1(blk := to_share \<circ> idx \<^enum>\<^sub>m (map_option nosep \<circ> Map_of_Val u_idx)) \<Ztypecolon> \<phi> Identity \<longmapsto>
+        \<lambda>\<r>\<e>\<t>. 1(blk := to_share \<circ> idx \<^enum>\<^sub>m (map_option nosep \<circ> Map_of_Val v)) \<Ztypecolon> \<phi> Identity \<rbrace> \<close>
+  by (rule "_setter_rule_2_"[where f=\<open>Some \<circ> map_nosep (index_mod_value idx (\<lambda>_. v))\<close>
+                        and V=\<open>nosep ` {a. index_value idx a = u_idx}\<close>
+                        and F=\<open>\<lambda>_. to_share o idx \<^enum>\<^sub>m (map_option nosep \<circ> Map_of_Val v)\<close>
+                        for idx v u_idx,
+                      OF fiction_Map_of_Val_perm_partial_refinement
+                         fiction_Map_of_Val_ins_perm_projection],
+      assumption,
+      assumption,
+      assumption,
+      assumption,
+      assumption,
+      simp add: split_nosep_meta_all inj_image_mem_iff index_mod_value_welltyp)
+
+lemma deallocate_rule:
+  \<open> v \<in> Well_Type (typ_of_blk blk)
+\<Longrightarrow> \<p>\<r>\<o>\<c> R.\<phi>R_set_res' (map_fun_at blk Map.empty)
+      \<lbrace> 1(blk := to_share \<circ> (map_option nosep \<circ> Map_of_Val v)) \<Ztypecolon> \<phi> Identity \<longmapsto>
+        \<lambda>\<r>\<e>\<t>. 1 \<Ztypecolon> \<phi> Identity \<rbrace> \<close>
+subgoal premises prems
+proof -
+  have [simp]:
+    \<open>Map.empty \<circ> the = Map.empty\<close>
+    unfolding fun_eq_iff by simp
+
+  note inj_image_mem_iff[simp] pointwise_set_UNIV[simp] \<F>_functional_condition_Map_of_Val_ins_dom[simp]
+       \<F>_functional_comp[where f=\<open>(\<circ>) to_share\<close> and Df=\<open>UNIV\<close>, simplified, symmetric, simp]
+
+  show ?thesis
+    by (rule "_setter_rule_2_"[where f=\<open>\<lambda>_. None\<close> and V=\<open>{nosep v}\<close> and F=\<open>\<lambda>_. 1\<close> for v, simplified],
+        unfold refinement_source_subjection, rule impI,
+        rule sep_refinement_stepwise[
+                  OF refinement_frame[OF Map_of_Val_ins.\<F>_functional_refinement[simplified]]
+                     pointwise_to_share.\<F>_functional_refinement
+                     pointwise_to_share.\<F>_functional_projection,
+                  where a4=\<open>Some (nosep u)\<close> and b4=None for u,
+                  simplified],
+        simp add: Map_of_Val_ins_dom_def,
+
+        rule refinement_projections_stepwise_UNIV_paired[
+          OF Map_of_Val_ins.\<F>_functional_projection
+             pointwise_to_share.\<F>_functional_projection,
+          where Dc=\<open>{Some (nosep v)}\<close>,
+          simplified],
+        rule prems)
+qed .
+
+end
 
 end
