Phi_Semantics/PhiSem_Mem_C_Tuple.thy
@@ -3,7 +3,7 @@ theory PhiSem_Mem_C_Tuple
 begin
 
 debt_axiomatization
-    Mapof_Val_tup: \<open>Mapof_Val (V_tup.mk vs) = nnode (map Mapof_Val vs)\<close>
+    Map_of_Val_tup: \<open>Map_of_Val (V_tup.mk vs) = nnode (map Map_of_Val vs)\<close>
 
 
 end
