Phi_Semantics_Framework/Resource_Space_Inst_Tools.thy
@@ -121,25 +121,29 @@ lemma In_1[simp]:
   \<open>sum1.Inr 1 = 1\<close>
   by (transfer; simp)+
 
-interpretation left: sep_insertion sum1.Inl sum1.projl
+interpretation left: sep_inj_proj sum1.Inl sum1.projl
   apply (standard; transfer)
+  apply (simp)
   apply (simp)
   apply (simp)
   apply (case_tac x; case_tac y; simp; meson)
     apply (case_tac a; case_tac b; simp; meson; simp)
     apply simp
+  apply simp
 apply simp
 apply (case_tac a; case_tac b; simp; meson; simp)
   by blast
 
-interpretation right: sep_insertion sum1.Inr sum1.projr
+interpretation right: sep_inj_proj sum1.Inr sum1.projr
   apply (standard; transfer)
+  apply (simp)
   apply (simp)
   apply (simp)
   apply (case_tac x; case_tac y; simp; meson)
     apply (case_tac a; case_tac b; simp; meson; simp)
     apply simp
-apply simp
+  apply simp
+apply (simp)
 apply (case_tac a; case_tac b; simp; meson; simp)
   by blast
 
