Phi_System/Fiction_Refinement.thy
@@ -6,7 +6,7 @@ begin
 
 
 
-
+ 
 
 
 
@@ -96,13 +96,13 @@ lemma
 
 (*
 lemma
-  \<open>refinement_projection I1 (refinement_projection I2 (UNIV * D)) \<subseteq> refinement_projection (I1 o\<^sub>\<I> I2) D\<close>
+  \<open>refinement_projection I1 (refinement_projection I2 (UNIV * D)) \<subseteq> refinement_projection (I1 ;\<^sub>\<I> I2) D\<close>
 unfolding refinement_projection_def
   apply (clarsimp simp add: Bex_def set_eq_iff set_mult_expn)
   subgoal for x u v u' v'
 
 lemma
-  \<open>refinement_projection (I1 o\<^sub>\<I> I2) D \<subseteq> refinement_projection I1 (refinement_projection I2 D)\<close>
+  \<open>refinement_projection (I1 ;\<^sub>\<I> I2) D \<subseteq> refinement_projection I1 (refinement_projection I2 D)\<close>
   for I1 :: \<open>('c::sep_monoid, 'a::sep_magma_1) interp\<close>
   unfolding refinement_projection_def
   apply (clarsimp simp add: Bex_def set_eq_iff set_mult_expn)
@@ -169,7 +169,7 @@ context begin
 
 private lemma from_fictional_refinement':
   \<open> Valid_Proc f
-\<Longrightarrow> (\<And>v. Transition_of' f v \<r>\<e>\<f>\<i>\<n>\<e>\<s> Rel v \<w>.\<r>.\<t> R.basic_fiction o\<^sub>\<I> I \<i>\<n> D)
+\<Longrightarrow> (\<And>v. Transition_of' f v \<r>\<e>\<f>\<i>\<n>\<e>\<s> Rel v \<w>.\<r>.\<t> R.basic_fiction ;\<^sub>\<I> I \<i>\<n> D)
 \<Longrightarrow> Valid_Transition Rel
 \<Longrightarrow> x \<in> D
 \<Longrightarrow> \<p>\<r>\<o>\<c> f \<lbrace> x \<Ztypecolon> \<phi> Identity \<longmapsto> \<lambda>v. y \<Ztypecolon> \<phi> Identity \<s>\<u>\<b>\<j> y. (x,y) \<in> Rel (Normal v) \<rbrace> \<t>\<h>\<r>\<o>\<w>\<s> (\<lambda>e. y \<Ztypecolon> \<phi> Identity \<s>\<u>\<b>\<j> y. (x,y) \<in> Rel (Abnm e))\<close>
@@ -216,7 +216,7 @@ lemma from_fictional_refinement:
   \<open> Valid_Proc f
 \<Longrightarrow> YY = (\<lambda>v. y \<Ztypecolon> \<phi> Identity \<s>\<u>\<b>\<j> y. (x,y) \<in> Rel (Normal v))
 \<Longrightarrow> EE = (\<lambda>e. y \<Ztypecolon> \<phi> Identity \<s>\<u>\<b>\<j> y. (x,y) \<in> Rel (Abnm e))
-\<Longrightarrow> (\<And>v. Transition_of' f v \<r>\<e>\<f>\<i>\<n>\<e>\<s> Rel v \<w>.\<r>.\<t> R.basic_fiction o\<^sub>\<I> I \<i>\<n> D)
+\<Longrightarrow> (\<And>v. Transition_of' f v \<r>\<e>\<f>\<i>\<n>\<e>\<s> Rel v \<w>.\<r>.\<t> R.basic_fiction ;\<^sub>\<I> I \<i>\<n> D)
 \<Longrightarrow> Valid_Transition Rel
 \<Longrightarrow> x \<in> D
 \<Longrightarrow> \<p>\<r>\<o>\<c> f \<lbrace> x \<Ztypecolon> \<phi> Identity \<longmapsto> YY \<rbrace> \<t>\<h>\<r>\<o>\<w>\<s> EE\<close>
@@ -226,7 +226,7 @@ end
 
 lemma "__getter_rule__":
   \<open> Valid_Proc getter
-\<Longrightarrow> (\<And>ret. Transition_of' getter ret \<r>\<e>\<f>\<i>\<n>\<e>\<s> Id_on ({x} \<s>\<u>\<b>\<j> ret = Normal (\<phi>arg v)) \<w>.\<r>.\<t> R.basic_fiction o\<^sub>\<I> I \<i>\<n> {x})
+\<Longrightarrow> (\<And>ret. Transition_of' getter ret \<r>\<e>\<f>\<i>\<n>\<e>\<s> Id_on ({x} \<s>\<u>\<b>\<j> ret = Normal (\<phi>arg v)) \<w>.\<r>.\<t> R.basic_fiction ;\<^sub>\<I> I \<i>\<n> {x})
 \<Longrightarrow> \<p>\<r>\<o>\<c> getter \<lbrace> x \<Ztypecolon> \<phi> Identity \<longmapsto> \<lambda>ret. x \<Ztypecolon> \<phi> Identity \<s>\<u>\<b>\<j> ret = \<phi>arg v \<rbrace>\<close>
   by (rule from_fictional_refinement[where Rel = \<open>\<lambda>ret. Id_on ({x} \<s>\<u>\<b>\<j> ret = Normal (\<phi>arg v))\<close>
                                        and D = \<open>{x}\<close>],
@@ -240,7 +240,7 @@ lemma "__getter_rule__":
 lemma "__setter_rule__":
   \<open> Valid_Proc setter
 \<Longrightarrow> (\<And>ret. Transition_of' setter ret \<r>\<e>\<f>\<i>\<n>\<e>\<s> {(x,y)} \<s>\<u>\<b>\<j> ret = Normal \<phi>V_none
-            \<w>.\<r>.\<t> R.basic_fiction o\<^sub>\<I> I \<i>\<n> {x})
+            \<w>.\<r>.\<t> R.basic_fiction ;\<^sub>\<I> I \<i>\<n> {x})
 \<Longrightarrow> \<p>\<r>\<o>\<c> setter \<lbrace> x \<Ztypecolon> \<phi> Identity \<longmapsto> \<lambda>_. y \<Ztypecolon> \<phi> Identity \<rbrace>\<close>
   by (rule from_fictional_refinement
                   [where Rel=\<open>\<lambda>ret. {(x,y)} \<s>\<u>\<b>\<j> ret = Normal \<phi>V_none\<close> and D = \<open>{x}\<close>],
@@ -254,7 +254,7 @@ lemma "__setter_rule__":
 lemma "__allocator_rule__":
   \<open> Valid_Proc allocator
 \<Longrightarrow> (\<And>ret. Transition_of' allocator ret \<r>\<e>\<f>\<i>\<n>\<e>\<s> {(1,y k)} \<s>\<u>\<b>\<j> k. ret = Normal (\<phi>arg k) \<and> P k
-            \<w>.\<r>.\<t> R.basic_fiction o\<^sub>\<I> I \<i>\<n> {1})
+            \<w>.\<r>.\<t> R.basic_fiction ;\<^sub>\<I> I \<i>\<n> {1})
 \<Longrightarrow> \<p>\<r>\<o>\<c> allocator \<lbrace> Void \<longmapsto> \<lambda>ret. y k \<Ztypecolon> \<phi> Identity \<s>\<u>\<b>\<j> k. ret = \<phi>arg k \<and> P k \<rbrace>\<close>
   by (rule from_fictional_refinement
         [where Rel=\<open>\<lambda>ret. {(1,y k)} \<s>\<u>\<b>\<j> k. ret = Normal (\<phi>arg k) \<and> P k\<close>
@@ -488,7 +488,7 @@ subsubsection \<open>pointwise_fiction_for_partial_mapping_resource\<close>
 
 locale pointwise_fiction_for_partial_mapping_resource =
    R: partial_map_resource Res
-+  fiction_kind FIC.DOMAIN INTERPRET Fic \<open>R.basic_fiction o\<^sub>\<I> \<F>_pointwise I\<close>
++  fiction_kind FIC.DOMAIN INTERPRET Fic \<open>R.basic_fiction ;\<^sub>\<I> \<F>_pointwise I\<close>
 for Res :: "('key \<Rightarrow> 'val::nonsepable_semigroup option) resource_entry"
 and I :: \<open>('fic::sep_algebra, 'val option) interp\<close>
 and Fic :: "('key \<Rightarrow> 'fic) fiction_entry"
@@ -542,7 +542,7 @@ subsubsection \<open>pointwise_fiction_for_two_level_partial_mapping_resource\<c
 
 locale pointwise_fiction_for_two_level_partial_mapping_resource =
    R: partial_map_resource2 Res
-+  fiction_kind FIC.DOMAIN INTERPRET Fic \<open>R.basic_fiction o\<^sub>\<I> \<F>_pointwise (\<F>_pointwise I)\<close>
++  fiction_kind FIC.DOMAIN INTERPRET Fic \<open>R.basic_fiction ;\<^sub>\<I> \<F>_pointwise (\<F>_pointwise I)\<close>
 for Res :: "('key \<Rightarrow> 'key2 \<Rightarrow> 'val::nonsepable_semigroup option) resource_entry"
 and I :: \<open>('fic::sep_algebra, 'val option) interp\<close>
 and Fic :: "('key \<Rightarrow> 'key2 \<Rightarrow> 'fic) fiction_entry"
@@ -607,7 +607,7 @@ end
 
 term \<open>(o) f\<close>
 
-term \<open>(o\<^sub>\<I>) I\<close>
+term \<open>(;\<^sub>\<I>) I\<close>
 
 lemma
   \<open>Id_on UNIV * Id_on {u} \<r>\<e>\<f>\<i>\<n>\<e>\<s> Id_on {f u} \<w>.\<r>.\<t> I \<i>\<n> {f u}\<close>
